@prefix : <https://w3id.org/won/message#> .
@prefix dc: <http://purl.org/dc/elements/1.1/> .
@prefix owl: <http://www.w3.org/2002/07/owl#> .
@prefix rdf: <http://www.w3.org/1999/02/22-rdf-syntax-ns#> .
@prefix xml: <http://www.w3.org/XML/1998/namespace> .
@prefix xsd: <http://www.w3.org/2001/XMLSchema#> .
@prefix rdfs: <http://www.w3.org/2000/01/rdf-schema#> .
@base <https://w3id.org/won/message> .

<https://w3id.org/won/message> rdf:type owl:Ontology ;
                                     
                                     dc:date "2013-12-13"^^xsd:date ;
                                     
                                     dc:creator "Yana Panchenko" ,
                                                "Fabian Salcher" ,
                                                "Florian Kleedorfer" ;
                                     
                                     rdfs:comment "Ontology for describing messages in the Web of Needs project."@en ;
                                     
                                     dc:title "Web of Needs Ontology"@en ;
                                     
                                     owl:versionIRI <https://w3id.org/won/message/1.0> .


#################################################################
#
#    Object Properties
#
#################################################################


###  https://w3id.org/won/message#content

:content rdf:type owl:ObjectProperty ;
            
            rdfs:comment "Points to an RDF graph URI that contains the message payload."@en ;
            
            rdfs:isDefinedBy <https://w3id.org/won/message> .



###  https://w3id.org/won/message#messageType

:messageType rdf:type owl:ObjectProperty ;
                
                rdfs:comment "Indicates the type of the message."@en ;
                
                rdfs:isDefinedBy <https://w3id.org/won/message> .



###  https://w3id.org/won/message#recipient

:recipient rdf:type owl:ObjectProperty ;
             
             rdfs:comment "Indicates the receiver of the message, either Socket or Connection."@en ;
             
             rdfs:isDefinedBy <https://w3id.org/won/message> .



###  https://w3id.org/won/message#recipientAtom

:recipientAtom rdf:type owl:ObjectProperty ;
                 
                 rdfs:comment "Indicates the Atom that 'contains' the receiver of the message."@en ;
                 
                 rdfs:isDefinedBy <https://w3id.org/won/message> .



###  https://w3id.org/won/message#recipientNode

:recipientNode rdf:type owl:ObjectProperty ;
                 
                 rdfs:comment "Indicates the WoN Node the message recipient is hosted on."@en ;
                 
                 rdfs:isDefinedBy <https://w3id.org/won/message> .



###  https://w3id.org/won/message#responseStateProperty

:responseStateProperty rdf:type owl:ObjectProperty ;
                          
                          rdfs:comment "Indicates the response state of a message."@en ;
                          
                          rdfs:isDefinedBy <https://w3id.org/won/message> ;
                          
                          rdfs:range :ResponseState .



###  https://w3id.org/won/message#sender

:sender rdf:type owl:ObjectProperty ;
           
           rdfs:comment "Indicates the sender of the message."@en ;
           
           rdfs:isDefinedBy <https://w3id.org/won/message> .



###  https://w3id.org/won/message#senderAtom

:senderAtom rdf:type owl:ObjectProperty ;
               
               rdfs:comment "Indicates the Atom that 'contains' the sender of the message."@en ;
               
               rdfs:isDefinedBy <https://w3id.org/won/message> .



###  https://w3id.org/won/message#senderNode

:senderNode rdf:type owl:ObjectProperty ;
               
               rdfs:comment "Indicates the WoN Node the message sender is hosted on."@en ;
               
               rdfs:isDefinedBy <https://w3id.org/won/message> .



###  https://w3id.org/won/message#newAtomState

:newAtomState rdf:type owl:ObjectProperty ;
              
              rdfs:comment "Used in an Activate/Deactivate message to indicate the new state the atom is to be moved to."@en ;
              
              rdfs:isDefinedBy <https://w3id.org/won/message> .



###  https://w3id.org/won/message#refersTo

:refersTo rdf:type owl:ObjectProperty ;
          
          rdfs:comment "Points to another message. Messages always exist in two copies: one on the sender's WoN node and one on the receiver's WoN node. The receiver's WoN node copies the message, mints a new URI for it and points to the original message using 'msg:refersTo'. In case of a forwarded message, this property points to the original message."@en ;
          
          rdfs:isDefinedBy <https://w3id.org/won/message> .





#################################################################
#
#    Data properties
#
#################################################################


###  https://w3id.org/won/message#timestamp

:timestamp rdf:type owl:DatatypeProperty ;
              
              rdfs:comment "Holds the timestamp assigned when the WoN node created the message."@en ;
              
              rdfs:isDefinedBy <https://w3id.org/won/message> .





#################################################################
#
#    Classes
#
#################################################################


###  https://w3id.org/won/message#ActivateMessage

:ActivateMessage rdf:type owl:Class ;
                 
                 rdfs:subClassOf :MessageType ;
                 
                 rdfs:comment "Type of message that activates an Atom."@en ;
                 
                 rdfs:isDefinedBy <https://w3id.org/won/message> .



###  https://w3id.org/won/message#CloseMessage

:CloseMessage rdf:type owl:Class ;
              
              rdfs:subClassOf :MessageType ;
              
              rdfs:comment "Type of message that closes a Connection."@en ;
              
              rdfs:isDefinedBy <https://w3id.org/won/message> .



###  https://w3id.org/won/message#ConnectMessage

:ConnectMessage rdf:type owl:Class ;
                
                rdfs:subClassOf :MessageType ;
                
                rdfs:comment "Type of message that is sent from Atom A to Atom B in order to create a new Connection."@en ;
                
                rdfs:isDefinedBy <https://w3id.org/won/message> .



###  https://w3id.org/won/message#ConnectionMessage

:ConnectionMessage rdf:type owl:Class ;
                   
                   rdfs:subClassOf :MessageType ;
                   
                   rdfs:comment "Message sent via an established connection. This type is to be used in Socket-specific protocols."@en ;
                   
                   rdfs:isDefinedBy <https://w3id.org/won/message> .

###  https://w3id.org/won/message#AtomMessage

:AtomMessage rdf:type owl:Class ;

                   rdfs:subClassOf :MessageType ;

                   rdfs:comment "Message sent between an atom's owner and the WoN node hosting the atom. The message is informative only
                   and has no side effect The message is not routed to any other participant."@en ;

                   rdfs:isDefinedBy <https://w3id.org/won/message> .


###  https://w3id.org/won/message#CreateMessage

:CreateMessage rdf:type owl:Class ;
               
               rdfs:subClassOf :MessageType ;
               
               rdfs:comment "Type of message sent to a WoN Node in order to create a new Atom."@en ;
               
               rdfs:isDefinedBy <https://w3id.org/won/message> .

			   
###  https://w3id.org/won/message#ReplaceMessage

:ReplaceMessage rdf:type owl:Class ;
               
               rdfs:subClassOf :MessageType ;
               
               rdfs:comment "Type of message sent to a WoN Node in order replace an Atom's content."@en ;
               
               rdfs:isDefinedBy <https://w3id.org/won/message> .
			   

###  https://w3id.org/won/message#ChangeNotificationMessage

:ChangeNotificationMessage rdf:type owl:Class ;

               rdfs:subClassOf :MessageType ;

               rdfs:comment "Type of message sent from a WoN Node to indicate that the remote Atom has changed."@en ;

               rdfs:isDefinedBy <https://w3id.org/won/message> .


###  https://w3id.org/won/message#DeactivateMessage

:DeactivateMessage rdf:type owl:Class ;
                   
                   rdfs:subClassOf :MessageType ;
                   
                   rdfs:comment "Type of message that deactivates an Atom."@en ;
                   
                   rdfs:isDefinedBy <https://w3id.org/won/message> .



###  https://w3id.org/won/message#EnvelopeGraph

:EnvelopeGraph rdf:type owl:Class ;
               
               rdfs:comment "Used to define the type of an RDF graph URI so as to explicitly mark it as an envelope graph. An Envelope contains the addressing information."@en ;
               
               rdfs:isDefinedBy <https://w3id.org/won/message> .



###  https://w3id.org/won/message#ForwardedEnvelopeGraph

:ForwardedEnvelopeGraph rdf:type owl:Class ;
                        
                        rdfs:subClassOf :EnvelopeGraph ;
                        
                        rdfs:comment "Used to define the type of an RDF graph URI so as to explicitly mark it as a forwarded envelope graph. The graph is expected to contain the original addressing information of a forwarded message."@en ;
                        
                        rdfs:isDefinedBy <https://w3id.org/won/message> .



###  https://w3id.org/won/message#HintMessage

:HintMessage rdf:type owl:Class ;
             
             rdfs:subClassOf :MessageType ;
             
             rdfs:comment "Type of message sent by a matching service to an Atom in order to inform its owner of other Atoms possibly interesting for establishing a connection."@en ;
             
             rdfs:isDefinedBy <https://w3id.org/won/message> .



###  https://w3id.org/won/message#MessageType

:MessageType rdf:type owl:Class ;
             
             rdfs:comment "Superclass of all WoN messages"@en ;
             
             rdfs:isDefinedBy <https://w3id.org/won/message> .



###  https://w3id.org/won/message#OpenMessage

:OpenMessage rdf:type owl:Class ;
             
             rdfs:subClassOf :MessageType ;
             
             rdfs:comment "Type of Message used to (re)open an existing Connection."@en ;
             
             rdfs:isDefinedBy <https://w3id.org/won/message> .



###  https://w3id.org/won/message#ResponseState

:ResponseState rdf:type owl:Class ;
               
               rdfs:comment "Indicates the (success/error) state of a response message."@en ;
               
               rdfs:isDefinedBy <https://w3id.org/won/message> .





#################################################################
#
#    Individuals
#
#################################################################


###  https://w3id.org/won/message#FailureResponse

:FailureResponse rdf:type :ResponseState ,
                          owl:NamedIndividual ;
                 
                 rdfs:comment "Indicates an error occurred while processing the message."@en ;
                 
                 rdfs:isDefinedBy <https://w3id.org/won/message> .



###  https://w3id.org/won/message#SuccessResponse

:SuccessResponse rdf:type :ResponseState ,
                          owl:NamedIndividual ;
                 
                 rdfs:comment "Indicates that the message was processed successfully."@en ;
                 
                 rdfs:isDefinedBy <https://w3id.org/won/message> .




###  Generated by the OWL API (version 3.4.2) http://owlapi.sourceforge.net

