@prefix : <http://purl.org/webofneeds/message#> .
@prefix dc: <http://purl.org/dc/elements/1.1/> .
@prefix owl: <http://www.w3.org/2002/07/owl#> .
@prefix rdf: <http://www.w3.org/1999/02/22-rdf-syntax-ns#> .
@prefix xml: <http://www.w3.org/XML/1998/namespace> .
@prefix xsd: <http://www.w3.org/2001/XMLSchema#> .
@prefix rdfs: <http://www.w3.org/2000/01/rdf-schema#> .
@base <http://purl.org/webofneeds/message> .

<http://purl.org/webofneeds/message> rdf:type owl:Ontology ;
                                     
                                     dc:date "2013-12-13"^^xsd:date ;
                                     
                                     dc:creator "Yana Panchenko" ,
                                                "Fabian Salcher" ,
                                                "Florian Kleedorfer" ;
                                     
                                     rdfs:comment "Ontology for describing messages in the Web of Needs project."@en ;
                                     
                                     dc:title "Web of Needs Ontology"@en ;
                                     
                                     owl:versionIRI <http://purl.org/webofneeds/message/1.0> .


#################################################################
#
#    Object Properties
#
#################################################################


###  http://purl.org/webofneeds/message#hasContent

:hasContent rdf:type owl:ObjectProperty ;
            
            rdfs:comment "Points to an RDF graph URI that contains the message payload."@en ;
            
            rdfs:isDefinedBy <http://purl.org/webofneeds/message> .



###  http://purl.org/webofneeds/message#hasMessageType

:hasMessageType rdf:type owl:ObjectProperty ;
                
                rdfs:comment "Indicates the type of the message."@en ;
                
                rdfs:isDefinedBy <http://purl.org/webofneeds/message> .



###  http://purl.org/webofneeds/message#hasReceiver

:hasReceiver rdf:type owl:ObjectProperty ;
             
             rdfs:comment "Indicates the receiver of the message, either Facet or Connection."@en ;
             
             rdfs:isDefinedBy <http://purl.org/webofneeds/message> .



###  http://purl.org/webofneeds/message#hasReceiverNeed

:hasReceiverNeed rdf:type owl:ObjectProperty ;
                 
                 rdfs:comment "Indicates the Need that 'contains' the receiver of the message."@en ;
                 
                 rdfs:isDefinedBy <http://purl.org/webofneeds/message> .



###  http://purl.org/webofneeds/message#hasReceiverNode

:hasReceiverNode rdf:type owl:ObjectProperty ;
                 
                 rdfs:comment "Indicates the WoN Node the message recipient is hosted on."@en ;
                 
                 rdfs:isDefinedBy <http://purl.org/webofneeds/message> .



###  http://purl.org/webofneeds/message#hasResponseStateProperty

:hasResponseStateProperty rdf:type owl:ObjectProperty ;
                          
                          rdfs:comment "Indicates the response state of a message."@en ;
                          
                          rdfs:isDefinedBy <http://purl.org/webofneeds/message> ;
                          
                          rdfs:range :ResponseState .



###  http://purl.org/webofneeds/message#hasSender

:hasSender rdf:type owl:ObjectProperty ;
           
           rdfs:comment "Indicates the sender of the message."@en ;
           
           rdfs:isDefinedBy <http://purl.org/webofneeds/message> .



###  http://purl.org/webofneeds/message#hasSenderNeed

:hasSenderNeed rdf:type owl:ObjectProperty ;
               
               rdfs:comment "Indicates the Need that 'contains' the sender of the message."@en ;
               
               rdfs:isDefinedBy <http://purl.org/webofneeds/message> .



###  http://purl.org/webofneeds/message#hasSenderNode

:hasSenderNode rdf:type owl:ObjectProperty ;
               
               rdfs:comment "Indicates the WoN Node the message sender is hosted on."@en ;
               
               rdfs:isDefinedBy <http://purl.org/webofneeds/message> .



###  http://purl.org/webofneeds/message#newNeedState

:newNeedState rdf:type owl:ObjectProperty ;
              
              rdfs:comment "Used in an Activate/Deactivate message to indicate the new state the need is to be moved to."@en ;
              
              rdfs:isDefinedBy <http://purl.org/webofneeds/message> .



###  http://purl.org/webofneeds/message#refersTo

:refersTo rdf:type owl:ObjectProperty ;
          
          rdfs:comment "Points to another message. Messages always exist in two copies: one on the sender's WoN node and one on the receiver's WoN node. The receiver's WoN node copies the message, mints a new URI for it and points to the original message using 'msg:refersTo'. In case of a forwarded message, this property points to the original message."@en ;
          
          rdfs:isDefinedBy <http://purl.org/webofneeds/message> .





#################################################################
#
#    Data properties
#
#################################################################


###  http://purl.org/webofneeds/message#hasTimestamp

:hasTimestamp rdf:type owl:DatatypeProperty ;
              
              rdfs:comment "Holds the timestamp assigned when the WoN node created the message."@en ;
              
              rdfs:isDefinedBy <http://purl.org/webofneeds/message> .





#################################################################
#
#    Classes
#
#################################################################


###  http://purl.org/webofneeds/message#ActivateMessage

:ActivateMessage rdf:type owl:Class ;
                 
                 rdfs:subClassOf :MessageType ;
                 
                 rdfs:comment "Type of message that activates a Need."@en ;
                 
                 rdfs:isDefinedBy <http://purl.org/webofneeds/message> .



###  http://purl.org/webofneeds/message#CloseMessage

:CloseMessage rdf:type owl:Class ;
              
              rdfs:subClassOf :MessageType ;
              
              rdfs:comment "Type of message that closes a Connection."@en ;
              
              rdfs:isDefinedBy <http://purl.org/webofneeds/message> .



###  http://purl.org/webofneeds/message#ConnectMessage

:ConnectMessage rdf:type owl:Class ;
                
                rdfs:subClassOf :MessageType ;
                
                rdfs:comment "Type of message that is sent from Need A to Need B in order to create a new Connection."@en ;
                
                rdfs:isDefinedBy <http://purl.org/webofneeds/message> .



###  http://purl.org/webofneeds/message#ConnectionMessage

:ConnectionMessage rdf:type owl:Class ;
                   
                   rdfs:subClassOf :MessageType ;
                   
                   rdfs:comment "Message sent via an established connection. This type is to be used in Facet-specific protocols."@en ;
                   
                   rdfs:isDefinedBy <http://purl.org/webofneeds/message> .

###  http://purl.org/webofneeds/message#NeedMessage

:NeedMessage rdf:type owl:Class ;

                   rdfs:subClassOf :MessageType ;

                   rdfs:comment "Message sent between a need's owner and the WoN node hosting the need. The message is informative only
                   and has no side effect The message is not routed to any other participant."@en ;

                   rdfs:isDefinedBy <http://purl.org/webofneeds/message> .


###  http://purl.org/webofneeds/message#CreateMessage

:CreateMessage rdf:type owl:Class ;
               
               rdfs:subClassOf :MessageType ;
               
               rdfs:comment "Type of message sent to a WoN Node in order to create a new Need."@en ;
               
               rdfs:isDefinedBy <http://purl.org/webofneeds/message> .

			   
###  http://purl.org/webofneeds/message#ReplaceMessage

:ReplaceMessage rdf:type owl:Class ;
               
               rdfs:subClassOf :MessageType ;
               
               rdfs:comment "Type of message sent to a WoN Node in order replace a Need's content."@en ;
               
               rdfs:isDefinedBy <http://purl.org/webofneeds/message> .
			   

###  http://purl.org/webofneeds/message#ChangeNotificationMessage

:ChangeNotificationMessage rdf:type owl:Class ;

               rdfs:subClassOf :MessageType ;

               rdfs:comment "Type of message sent from a WoN Node to indicate that the remote Need has changed."@en ;

               rdfs:isDefinedBy <http://purl.org/webofneeds/message> .


###  http://purl.org/webofneeds/message#DeactivateMessage

:DeactivateMessage rdf:type owl:Class ;
                   
                   rdfs:subClassOf :MessageType ;
                   
                   rdfs:comment "Type of message that deactivates a Need."@en ;
                   
                   rdfs:isDefinedBy <http://purl.org/webofneeds/message> .



###  http://purl.org/webofneeds/message#EnvelopeGraph

:EnvelopeGraph rdf:type owl:Class ;
               
               rdfs:comment "Used to define the type of an RDF graph URI so as to explicitly mark it as an envelope graph. An Envelope contains the addressing information."@en ;
               
               rdfs:isDefinedBy <http://purl.org/webofneeds/message> .



###  http://purl.org/webofneeds/message#ForwardedEnvelopeGraph

:ForwardedEnvelopeGraph rdf:type owl:Class ;
                        
                        rdfs:subClassOf :EnvelopeGraph ;
                        
                        rdfs:comment "Used to define the type of an RDF graph URI so as to explicitly mark it as a forwarded envelope graph. The graph is expected to contain the original addressing information of a forwarded message."@en ;
                        
                        rdfs:isDefinedBy <http://purl.org/webofneeds/message> .



###  http://purl.org/webofneeds/message#HintMessage

:HintMessage rdf:type owl:Class ;
             
             rdfs:subClassOf :MessageType ;
             
             rdfs:comment "Type of message sent by a matching service to a Need in order to inform its owner of other Needs possibly interesting for establishing a connection."@en ;
             
             rdfs:isDefinedBy <http://purl.org/webofneeds/message> .



###  http://purl.org/webofneeds/message#MessageType

:MessageType rdf:type owl:Class ;
             
             rdfs:comment "Superclass of all WoN messages"@en ;
             
             rdfs:isDefinedBy <http://purl.org/webofneeds/message> .



###  http://purl.org/webofneeds/message#OpenMessage

:OpenMessage rdf:type owl:Class ;
             
             rdfs:subClassOf :MessageType ;
             
             rdfs:comment "Type of Message used to (re)open an existing Connection."@en ;
             
             rdfs:isDefinedBy <http://purl.org/webofneeds/message> .



###  http://purl.org/webofneeds/message#ResponseState

:ResponseState rdf:type owl:Class ;
               
               rdfs:comment "Indicates the (success/error) state of a response message."@en ;
               
               rdfs:isDefinedBy <http://purl.org/webofneeds/message> .





#################################################################
#
#    Individuals
#
#################################################################


###  http://purl.org/webofneeds/message#FailureResponse

:FailureResponse rdf:type :ResponseState ,
                          owl:NamedIndividual ;
                 
                 rdfs:comment "Indicates an error occurred while processing the message."@en ;
                 
                 rdfs:isDefinedBy <http://purl.org/webofneeds/message> .



###  http://purl.org/webofneeds/message#SuccessResponse

:SuccessResponse rdf:type :ResponseState ,
                          owl:NamedIndividual ;
                 
                 rdfs:comment "Indicates that the message was processed successfully."@en ;
                 
                 rdfs:isDefinedBy <http://purl.org/webofneeds/message> .




###  Generated by the OWL API (version 3.4.2) http://owlapi.sourceforge.net

