@prefix : <https://w3id.org/won/core#> .
@prefix dc: <http://purl.org/dc/elements/1.1/> .
@prefix owl: <http://www.w3.org/2002/07/owl#> .
@prefix rdf: <http://www.w3.org/1999/02/22-rdf-syntax-ns#> .
@prefix xml: <http://www.w3.org/XML/1998/namespace> .
@prefix xsd: <http://www.w3.org/2001/XMLSchema#> .
@prefix rdfs: <http://www.w3.org/2000/01/rdf-schema#> .
@prefix vaem: <http://www.linkedmodel.org/schema/vaem#> .
@prefix vann: <http://purl.org/vocab/vann/> .
@prefix terms: <http://purl.org/dc/terms/> .
@base <https://w3id.org/won/core> .

<https://w3id.org/won/core> rdf:type owl:Ontology ;
                             owl:versionIRI <https://w3id.org/won/core/1.0> ;
                             dc:abstract """The Web of Needs is a decentralized linked data application infrastructure for mediating cooperation in the broadest sense.

Based on append-only message logs, users (or other agents) publish and manage objects (*Atoms*). The main goal of publishing Atoms is to express interest in cooperation, for example by specifying something that is needed or being offered. However, Atoms can contain arbitrary data and thus be used to build general linked data knowledge graphs.

Atoms can establish *Connections*  with other Atoms, if both Atoms' owners agree to it.

Matching services can make suggestions which atoms to connect to. An Atom specifies 'Sockets' indicating the kinds of Connections it is prepared to establish."""@en ;
                             dc:creator "Fabian Salcher" ,
                                        "Florian Kleedorfer" ;
                             dc:title "Web of Needs Core Ontology" ;
                             terms:created "2013-12-13"^^xsd:date ;
                             terms:license <https://creativecommons.org/licenses/by/4.0/> ;
                             vann:preferredNamespacePrefix "won" ;
                             rdfs:comment "Ontology for the Web of Needs data model."@en .

#################################################################
#    Annotation properties
#################################################################

###  http://purl.org/dc/elements/1.1/abstract
dc:abstract rdf:type owl:AnnotationProperty .


###  http://purl.org/dc/elements/1.1/creator
dc:creator rdf:type owl:AnnotationProperty .


###  http://purl.org/dc/elements/1.1/date
dc:date rdf:type owl:AnnotationProperty .


###  http://purl.org/dc/elements/1.1/description
dc:description rdf:type owl:AnnotationProperty .


###  http://purl.org/dc/elements/1.1/title
dc:title rdf:type owl:AnnotationProperty .


###  http://purl.org/dc/terms/created
terms:created rdf:type owl:AnnotationProperty .


###  http://purl.org/dc/terms/license
terms:license rdf:type owl:AnnotationProperty .


###  http://purl.org/vocab/vann/preferredNamespacePrefix
vann:preferredNamespacePrefix rdf:type owl:AnnotationProperty .


###  http://www.linkedmodel.org/schema/vaem#rationale
vaem:rationale rdf:type owl:AnnotationProperty .


#################################################################
#    Datatypes
#################################################################

###  http://www.w3.org/2001/XMLSchema#duration
xsd:duration rdf:type rdfs:Datatype .


#################################################################
#    Object Properties
#################################################################

###  https://w3id.org/won/core#atomList
:atomList rdf:type owl:ObjectProperty ;
          rdfs:domain :Node ;
          rdfs:range :AtomContainer ;
          rdfs:comment "The Node's atoms, in a LDP-pageable container." ;
          rdfs:label "atomList" .


###  https://w3id.org/won/core#atomState
:atomState rdf:type owl:ObjectProperty ,
                    owl:FunctionalProperty ;
           rdfs:domain :Atom ;
           rdfs:range :AtomState ;
           rdfs:comment "Defines the Atom object's state."@en ;
           rdfs:isDefinedBy <https://w3id.org/won/core> ;
           rdfs:label "atomState" .


###  https://w3id.org/won/core#compatibleSocketDefinition
:compatibleSocketDefinition rdf:type owl:ObjectProperty ;
                            rdfs:domain :SocketDefinition ;
                            rdfs:range :SocketDefinition ;
                            rdfs:comment "Identifies another SocketDefinition that is compatible with this one. Connections with other kinds of sockets will not be allowed unless they are explicitly annotated."@en ;
                            rdfs:label "compatibleSocketDefinition" .


###  https://w3id.org/won/core#connectionState
:connectionState rdf:type owl:ObjectProperty ,
                          owl:FunctionalProperty ;
                 rdfs:domain :Connection ;
                 rdfs:range :ConnectionState ;
                 rdfs:comment "Indicates the state in which the Connection object is."@en ;
                 rdfs:isDefinedBy <https://w3id.org/won/core> ;
                 rdfs:label "connectionState" .

###  https://w3id.org/won/core#previousConnectionState
:previousConnectionState rdf:type owl:ObjectProperty ,
                          owl:FunctionalProperty ;
                 rdfs:domain :Connection ;
                 rdfs:range :previousConnectionState ;
                 rdfs:comment "Indicates the state in which the Connection was before the current one."@en ;
                 rdfs:isDefinedBy <https://w3id.org/won/core> ;
                 rdfs:label "previousConnectionState" .

###  https://w3id.org/won/core#connections
:connections rdf:type owl:ObjectProperty ;
             rdfs:domain :Atom ;
             rdfs:range :ConnectionContainer ;
             rdfs:comment "Links the Atom object to its connections."@en ;
             rdfs:isDefinedBy <https://w3id.org/won/core> ;
             rdfs:label "connections" .


###  https://w3id.org/won/core#contentGraph
:contentGraph rdf:type owl:ObjectProperty ;
              rdfs:domain :Atom ;
              rdfs:range owl:Thing ;
              rdfs:comment "Links an Atom to an RDF graph holding some of its RDF content."@en ;
              rdfs:label "contentGraph" .


###  https://w3id.org/won/core#defaultSocket
:defaultSocket rdf:type owl:ObjectProperty ;
               rdfs:domain :Atom ;
               rdfs:range :Socket ;
               rdfs:comment "Indicates the socket to connect to by default."@en ;
               rdfs:isDefinedBy <https://w3id.org/won/core> ;
               rdfs:label "defaultSocket" .


###  https://w3id.org/won/core#derivesAtomProperty
:derivesAtomProperty rdf:type owl:ObjectProperty ;
                     rdfs:domain :SocketDefinition ;
                     rdfs:range rdf:Property ;
                     rdfs:comment "Defines a property to be 'derived' when the connection is established. The property will be used to derive a triple '[sourceAtom] [property] [targetAtom]'."@en ;
                     rdfs:label "derivesAtomProperty" .


###  https://w3id.org/won/core#derivesInverseAtomProperty
:derivesInverseAtomProperty rdf:type owl:ObjectProperty ;
                            rdfs:domain :SocketDefinition ;
                            rdfs:range rdf:Property ;
                            rdfs:comment "Defines a property to be 'derived' when the connection is established. The property will be used to derive a triple '[targetAtom] [property] [sourceAtom]'."@en ;
                            rdfs:label "derivesInverseAtomProperty" .


###  https://w3id.org/won/core#messageContainer
:messageContainer rdf:type owl:ObjectProperty ,
                           owl:FunctionalProperty ;
                  rdfs:domain [ rdf:type owl:Class ;
                                owl:unionOf ( :Atom
                                              :Connection
                                            )
                              ] ;
                  rdfs:range :MessageContainer ;
                  rdfs:comment "Links the Connection object to a container containing connection events (messages)."@en ;
                  rdfs:isDefinedBy <https://w3id.org/won/core> ;
                  rdfs:label "messageContainer" .


###  https://w3id.org/won/core#socket
:socket rdf:type owl:ObjectProperty ;
        rdfs:domain [ rdf:type owl:Class ;
                      owl:unionOf ( :Atom
                                    :Connection
                                  )
                    ] ;
        rdfs:range :Socket ;
        rdfs:comment "Indicates that an atom or connection supports the specified socket (=behavior)."@en ;
        rdfs:isDefinedBy <https://w3id.org/won/core> ;
        rdfs:label "socket" .


###  https://w3id.org/won/core#socketDefinition
:socketDefinition rdf:type owl:ObjectProperty ;
                  rdfs:domain :Socket ;
                  rdfs:range :SocketDefinition ;
                  rdfs:comment "Links the socket to its definition. A socket must have exactly one definition."@en ;
                  rdfs:label "socketDefinition" .


###  https://w3id.org/won/core#sourceAtom
:sourceAtom rdf:type owl:ObjectProperty ;
            rdfs:domain :Connection ;
            rdfs:range :Atom ;
            rdfs:comment "Links a Connection to the Atom it belongs to (the source of this Connection)"@en ;
            rdfs:label "sourceAtom" .


###  https://w3id.org/won/core#supportsWonProtocolImpl
:supportsWonProtocolImpl rdf:type owl:ObjectProperty ;
                         rdfs:domain :Node ;
                         rdfs:range :WonProtocol ;
                         rdfs:comment "Connects an WoN Node object with a description of a WON protocol it supports."@en ;
                         rdfs:isDefinedBy <https://w3id.org/won/core> ;
                         rdfs:label "supportsWonProtocolImpl" .


###  https://w3id.org/won/core#targetAtom
:targetAtom rdf:type owl:ObjectProperty ;
            rdfs:domain :Connection ;
            rdfs:range :Atom ;
            rdfs:comment "links a Connection to its remote Atom. The remote Atom is the one holding the  targetConnection."@en ;
            rdfs:isDefinedBy "https://w3id.org/won/core"@en ;
            rdfs:label "targetAtom" .


###  https://w3id.org/won/core#targetConnection
:targetConnection rdf:type owl:ObjectProperty ,
                           owl:FunctionalProperty ,
                           owl:InverseFunctionalProperty ,
                           owl:SymmetricProperty ;
                  rdfs:domain :Connection ;
                  rdfs:range :Connection ;
                  rdfs:comment "Links a Connection object to its remote counterpart."@en ;
                  rdfs:isDefinedBy <https://w3id.org/won/core> ;
                  rdfs:label "targetConnection" .


###  https://w3id.org/won/core#targetSocket
:targetSocket rdf:type owl:ObjectProperty ;
              rdfs:domain :Connection ;
              rdfs:range :Socket ;
              rdfs:comment "Indicates that a remote atom or remote connection supports the specified socket (=behavior) or specifies the remote socket to connect with."@en ;
              rdfs:isDefinedBy <https://w3id.org/won/core> ;
              rdfs:label "targetSocket" .


###  https://w3id.org/won/core#uriPrefixSpecification
:uriPrefixSpecification rdf:type owl:ObjectProperty ;
                        rdfs:domain :Node ;
                        rdfs:range :UriPrefixSpecification ;
                        rdfs:comment "Specification of URI prefixes used by this WoN node."@en ;
                        rdfs:label "uriPrefixSpecification" .


###  https://w3id.org/won/core#wonNode
:wonNode rdf:type owl:ObjectProperty ;
         rdfs:domain [ rdf:type owl:Class ;
                       owl:unionOf ( :Atom
                                     :Connection
                                   )
                     ] ;
         rdfs:range :Node ;
         rdfs:comment "Links an Atom or Connection to their WoN node."@en ;
         rdfs:label "wonNode" .


###  https://w3id.org/won/core#derivedForConnectionState
:derivedForConnectionState rdf:type owl:ObjectProperty ;
                           rdfs:domain :DerivedDataGraph ;
                           rdfs:range :ConnectionState ;
                           rdfs:comment "links a derived data graph to the connection state in which it was derived." ;
                           rdfs:label "derivedForConnectionState" .

#################################################################
#    Data properties
#################################################################

###  https://w3id.org/won/core#atomActivatedTopic
:atomActivatedTopic rdf:type owl:DatatypeProperty ;
                    rdfs:domain :WonOverActiveMq ;
                    rdfs:range xsd:string ;
                    rdfs:comment "The activeMQ topic to subscribe to to be informed when an atom is activated."@en ;
                    rdfs:label "atomActivatedTopic" .


###  https://w3id.org/won/core#atomCreatedTopic
:atomCreatedTopic rdf:type owl:DatatypeProperty ;
                  rdfs:domain :WonOverActiveMq ;
                  rdfs:range xsd:string ;
                  rdfs:comment "The activeMQ topic to subscribe to to be informed when an atom is created."@en ;
                  rdfs:label "atomCreatedTopic" .


###  https://w3id.org/won/core#atomDeactivatedTopic
:atomDeactivatedTopic rdf:type owl:DatatypeProperty ;
                      rdfs:domain :WonOverActiveMq ;
                      rdfs:range xsd:string ;
                      rdfs:comment "The activeMQ topic to subscribe to to be informed when an atom is deactivated."@en ;
                      rdfs:label "atomDeactivatedTopic" .


###  https://w3id.org/won/core#atomDeletedTopic
:atomDeletedTopic rdf:type owl:DatatypeProperty ;
                  rdfs:domain :WonOverActiveMq ;
                  rdfs:range xsd:string ;
                  rdfs:comment "The activeMQ topic to subscribe to to be informed when an atom is deleted."@en ;
                  rdfs:label "atomDeletedTopic" .


###  https://w3id.org/won/core#atomModifiedTopic
:atomModifiedTopic rdf:type owl:DatatypeProperty ;
                   rdfs:domain :WonOverActiveMq ;
                   rdfs:range xsd:string ;
                   rdfs:comment "The activeMQ topic to subscribe to to be informed when an atom is modified."@en ;
                   rdfs:label "atomModifiedTopic" .


###  https://w3id.org/won/core#atomUriPrefix
:atomUriPrefix rdf:type owl:DatatypeProperty ;
               rdfs:domain :UriPrefixSpecification ;
               rdfs:range xsd:string ;
               rdfs:comment "Specifies the prefix an atom must have on the node this specification applies to. This specification allows clients to generate new valid new Atom URIs."@en ;
               rdfs:label "atomUriPrefix" .


###  https://w3id.org/won/core#autoOpen
:autoOpen rdf:type owl:DatatypeProperty ;
          rdfs:domain :SocketDefinition ;
          rdfs:range xsd:boolean ;
          rdfs:comment "Indicates that any incoming CONNECT/OPEN message will be answered with OPEN unless the facet configuration forbids it."@en ;
          rdfs:label "autoOpen" .


###  https://w3id.org/won/core#brokerUri
:brokerUri rdf:type owl:DatatypeProperty ;
           rdfs:domain :WonOverActiveMq ;
           rdfs:range xsd:anyURI ;
           rdfs:comment "The URI of the activeMQ broker"@en ;
           rdfs:label "brokerUri" .


###  https://w3id.org/won/core#connectedCount
:connectedCount rdf:type owl:DatatypeProperty ;
                rdfs:domain :ConnectionContainer ;
                rdfs:range xsd:integer ;
                rdfs:comment "The number of connections in the container that are in state CONNECTED."@en ;
                rdfs:label "connectedCount".

###  https://w3id.org/won/core#suggestedCount
:suggestedCount rdf:type owl:DatatypeProperty ;
                rdfs:domain :ConnectionContainer ;
                rdfs:range xsd:integer ;
                rdfs:comment "The number of connections in the container that are in state SUGGESTED."@en ;
                rdfs:label "suggestedCount".

###  https://w3id.org/won/core#requestReceivedCount
:requestReceivedCount rdf:type owl:DatatypeProperty ;
                rdfs:domain :ConnectionContainer ;
                rdfs:range xsd:integer ;
                rdfs:comment "The number of connections in the container that are in state REQUEST_RECEIVED."@en ;
                rdfs:label "requestReceivedCount".

###  https://w3id.org/won/core#requestSentCount
:requestSentCount rdf:type owl:DatatypeProperty ;
                rdfs:domain :ConnectionContainer ;
                rdfs:range xsd:integer ;
                rdfs:comment "The number of connections in the container that are in state REQUEST_RECEIVED."@en ;
                rdfs:label "requestSentCount".

###  https://w3id.org/won/core#closedCount
:closedCount rdf:type owl:DatatypeProperty ;
                rdfs:domain :ConnectionContainer ;
                rdfs:range xsd:integer ;
                rdfs:comment "The number of connections in the container that are in state CLOSED."@en ;
                rdfs:label "closedCount".

###  https://w3id.org/won/core#connectionUriPrefix
:connectionUriPrefix rdf:type owl:DatatypeProperty ;
                     rdfs:domain :UriPrefixSpecification ;
                     rdfs:range xsd:string ;
                     rdfs:comment "Specifies the prefix a connection must have on the node this specification applies to."@en ;
                     rdfs:label "connectionUriPrefix" .


###  https://w3id.org/won/core#messageUriPrefix
:messageUriPrefix rdf:type owl:DatatypeProperty ;
                rdfs:domain :UriPrefixSpecification ;
                rdfs:range xsd:string ;
                rdfs:comment "Specifies the prefix a message must have on the node to which this specification applies. This specification allows clients to convert between a message URI (prefix 'wm:/') and a dereferencable https URI."@en ;
                rdfs:label "messageUriPrefix" .


###  https://w3id.org/won/core#matcherQueue
:matcherQueue rdf:type owl:DatatypeProperty ;
              rdfs:domain :WonOverActiveMq ;
              rdfs:range xsd:string ;
              rdfs:comment "The activeMQ queue to be used by matchers to send messages to the node."@en ;
              rdfs:label "matcherQueue" .


###  https://w3id.org/won/core#nodeQueue
:nodeQueue rdf:type owl:DatatypeProperty ;
           rdfs:domain :WonOverActiveMq ;
           rdfs:range xsd:string ;
           rdfs:comment "The activeMQ queue to be used by other nodes to send messages to the node."@en ;
           rdfs:label "nodeQueue" .


###  https://w3id.org/won/core#ownerQueue
:ownerQueue rdf:type owl:DatatypeProperty ;
            rdfs:domain :WonOverActiveMq ;
            rdfs:range xsd:string ;
            rdfs:comment "The activeMQ queue to be used by owners to send messages to the node."@en ;
            rdfs:label "ownerQueue" .


###  https://w3id.org/won/core#socketCapacity
:socketCapacity rdf:type owl:DatatypeProperty ;
                rdfs:domain :SocketDefinition ;
                rdfs:range xsd:integer ;
                rdfs:comment "Defines the maximum number of established connections supported by the socket."@en ;
                rdfs:label "socketCapacity" .


#################################################################
#    Classes
#################################################################

###  http://www.w3.org/1999/02/22-rdf-syntax-ns#Property
rdf:Property rdf:type owl:Class .


###  http://www.w3.org/ns/ldp#CompositeContainer
<http://www.w3.org/ns/ldp#CompositeContainer> rdf:type owl:Class ;
                                              rdfs:isDefinedBy <https://w3id.org/won/core> .


###  https://w3id.org/won/core#Atom
:Atom rdf:type owl:Class ;
      rdfs:comment """An atom is an online entity controlled by a person or organization. Its purpose is to be connected to other such atoms via Connections, so it can be said that it represents the need to interact with others.
It specifies a content - what the atom is about, which may be something that is offered for sale, sought for rental etc."""@en ;
      rdfs:isDefinedBy <https://w3id.org/won/core> ;
      rdfs:label "Atom" .


###  https://w3id.org/won/core#AtomContainer
:AtomContainer rdf:type owl:Class ;
               rdfs:subClassOf <http://www.w3.org/ns/ldp#CompositeContainer> ;
               rdfs:comment """An LDP container with all the Atoms stored on the Node.

The container supports LDP paging as described here: https://github.com/researchstudio-sat/webofneeds/blob/master/webofneeds/won-node-webapp/doc/linked-data-paging.md""" ;
               rdfs:label "AtomContainer" .


###  https://w3id.org/won/core#AtomState
:AtomState rdf:type owl:Class ;
           rdfs:comment "The Atom's state."@en ;
           rdfs:isDefinedBy <https://w3id.org/won/core> ;
           rdfs:label "AtomState" .


###  https://w3id.org/won/core#Connection
:Connection rdf:type owl:Class ;
            rdfs:comment "Represents a Connection to between two Atoms. Whenever two Atoms are connected, each Atom creates a dedicated Connection object which encapsulate all information about the connection."@en ;
            rdfs:isDefinedBy <https://w3id.org/won/core> ;
            rdfs:label "Connection" .


###  https://w3id.org/won/core#ConnectionContainer
:ConnectionContainer rdf:type owl:Class ;
                     rdfs:subClassOf <http://www.w3.org/ns/ldp#CompositeContainer> ;
                     owl:disjointWith :MessageContainer ;
                     rdfs:comment "Container for Connections. The container supports LDP paging as described here: https://github.com/researchstudio-sat/webofneeds/blob/master/webofneeds/won-node-webapp/doc/linked-data-paging.md"@en ;
                     rdfs:isDefinedBy <https://w3id.org/won/core> ;
                     rdfs:label "ConnectionContainer" .


###  https://w3id.org/won/core#ConnectionState
:ConnectionState rdf:type owl:Class ;
                 rdfs:comment "A Connection's state."@en ;
                 rdfs:isDefinedBy <https://w3id.org/won/core> ;
                 rdfs:label "ConnectionState" .


###  https://w3id.org/won/core#MessageContainer
:MessageContainer rdf:type owl:Class ;
                  rdfs:subClassOf <http://www.w3.org/ns/ldp#CompositeContainer> ;
                  rdfs:comment "Container for Messages. The container supports LDP paging as described here: https://github.com/researchstudio-sat/webofneeds/blob/master/webofneeds/won-node-webapp/doc/linked-data-paging.md."@en ;
                  rdfs:isDefinedBy <https://w3id.org/won/core> ;
                  rdfs:label "MessageContainer" .


###  https://w3id.org/won/core#Node
:Node rdf:type owl:Class ;
      rdfs:comment "A server storing Atoms and the data associated with them."@en ;
      rdfs:label "Node" .


###  https://w3id.org/won/core#Socket
:Socket rdf:type owl:Class ;
        rdfs:comment "An Atom defines how Connections can be established using any number of Socket individuals. Each connection between two Atoms must specify the Socket it is attached to on each side."@en ;
        rdfs:isDefinedBy <https://w3id.org/won/core> ;
        rdfs:label "Socket" .


###  https://w3id.org/won/core#SocketDefinition
:SocketDefinition rdf:type owl:Class ;
                  rdfs:comment "A Socket's definition."@en ;
                  rdfs:label "SocketDefinition" .


###  https://w3id.org/won/core#UriPrefixSpecification
:UriPrefixSpecification rdf:type owl:Class ;
                        rdfs:comment "Specification of URI prefixes for atoms, events, and connections for a WoN node."@en ;
                        rdfs:label "UriPrefixSpecification" .


###  https://w3id.org/won/core#WonOverActiveMq
:WonOverActiveMq rdf:type owl:Class ;
                 rdfs:subClassOf :WonProtocol ;
                 rdfs:comment "The Web of Needs protocol implementation that uses ActiveMQ."@en ;
                 rdfs:isDefinedBy <https://w3id.org/won/core> ;
                 rdfs:label "WonOverActiveMq" .


###  https://w3id.org/won/core#WonProtocol
:WonProtocol rdf:type owl:Class ;
             rdfs:comment "Superclass for Web of Needs protocol implementations."@en ;
             rdfs:isDefinedBy <https://w3id.org/won/core> ;
             rdfs:label "WonProtocol" .

###  https://w3id.org/won/core#DerivedDataGraph
:DerivedDataGraph rdf:type owl:Class ;
                  rdfs:label "DerivedDataGraph" ;
                  rdfs:isDefinedBy <https://w3id.org/won/core> ;
                  rdfs:comment "Graph of derived data." .

#################################################################
#    Individuals
#################################################################

###  https://w3id.org/won/core#Active
:Active rdf:type owl:NamedIndividual ,
                 :AtomState ;
        rdfs:comment "The active state. "@en ;
        rdfs:isDefinedBy <https://w3id.org/won/core> ;
        rdfs:label "Active" .


###  https://w3id.org/won/core#Closed
:Closed rdf:type owl:NamedIndividual ,
                 :ConnectionState ;
        rdfs:comment "The closed state. No Messages are forwarded in this state. Re-opening a connection is possbile."@en ;
        rdfs:isDefinedBy <https://w3id.org/won/core> ;
        rdfs:label "Closed" .


###  https://w3id.org/won/core#Connected
:Connected rdf:type owl:NamedIndividual ,
                    :ConnectionState ;
           rdfs:comment "The connected state. Messages are forwarded to/from the owner."@en ;
           rdfs:isDefinedBy <https://w3id.org/won/core> ;
           rdfs:label "Connected" .


###  https://w3id.org/won/core#Inactive
:Inactive rdf:type owl:NamedIndividual ,
                   :AtomState ;
          rdfs:comment "The incative state. Atoms do not communicate in this state. Intended to stop receiving messages for something not currently of interest."@en ;
          rdfs:isDefinedBy <https://w3id.org/won/core> ;
          rdfs:label "Inactive" .

###  https://w3id.org/won/core#Deleted
:Deleted rdf:type owl:NamedIndividual ,
                   :AtomState ;
          rdfs:comment "The deleted state. A deleted atom's URI is still remembered and associated with this state so that the WoN node can respond appropriately (410 GONE) when queried."@en ;
          rdfs:isDefinedBy <https://w3id.org/won/core> ;
          rdfs:label "Deleted" .

###  https://w3id.org/won/core#RequestReceived
:RequestReceived rdf:type owl:NamedIndividual ,
                          :ConnectionState ;
                 rdfs:comment "Half-open state. The connection has been opened by the remote counterpart but not yet been accepted by the local end."@en ;
                 rdfs:isDefinedBy <https://w3id.org/won/core> ;
                 rdfs:label "RequestReceived" .


###  https://w3id.org/won/core#RequestSent
:RequestSent rdf:type owl:NamedIndividual ,
                      :ConnectionState ;
             rdfs:comment "Half-open state. The Connection has been requested by the local end but not yet been accepted by the remote counterpart."@en ;
             rdfs:isDefinedBy <https://w3id.org/won/core> ;
             rdfs:label "RequestSent" .


###  https://w3id.org/won/core#Suggested
:Suggested rdf:type owl:NamedIndividual ,
                    :ConnectionState ;
           rdfs:comment "Suggested state. The Connection has been created through a Hint Event but not yet been opened by either of the sides."@en ;
           rdfs:isDefinedBy <https://w3id.org/won/core> ;
           rdfs:label "Suggested" .


#################################################################
#    General axioms
#################################################################

[ rdf:type owl:AllDifferent ;
  owl:distinctMembers rdf:nil
] .


###  Generated by the OWL API (version 4.5.9.2019-02-01T07:24:44Z) https://github.com/owlcs/owlapi
